src/StAM.v
@@ -4,13 +4,18 @@ Record representing the AM Monad state structure.
 Author:  Adam Petz, ampetz@ku.edu
 *)
 
-Require Import Maps.
+Require Import Maps_Class.
+Require Import Coq.Arith.EqNat.
 
-Definition BS := nat.
+(*Definition BS := nat. *)
+
+Instance nat_EqClass : EqClass nat :=
+  { eqb:= PeanoNat.Nat.eqb;
+    eqb_leibniz := beq_nat_true }.
 
 (* Specific AM monad state *)
 Record AM_St : Type := mkAM_St
-                         { am_nonceMap : Map (*Map nat BS*);
+                         { am_nonceMap : MapC nat nat;
                            am_nonceId : nat;
                            checked : list nat }.
                                          
